veric/initialize.v
@@ -1,0 +1,287 @@
+Load loadpath.
+Require Import veric.base.
+Require Import veric.Address.
+Require Import msl.rmaps.
+Require Import msl.rmaps_lemmas.
+Require Import veric.compcert_rmaps.
+Import Mem.
+Require Import msl.msl_standard.
+Require Import veric.juicy_mem veric.juicy_mem_lemmas veric.juicy_mem_ops.
+Require Import veric.res_predicates.
+Require Import veric.seplog.
+Require Import veric.assert_lemmas.
+Require Import veric.Clight_new.
+Require Import veric.expr veric.expr_lemmas.
+Require Import veric.Clight_lemmas.
+Require Import veric.initial_world.
+
+
+
+Lemma alloc_globals_app:
+   forall F V (ge: Genv.t F V) m m2 vs vs',
+  Genv.alloc_globals ge m (vs++vs') = Some m2 <->
+    exists m', Genv.alloc_globals ge m vs = Some m' /\
+                    Genv.alloc_globals ge m' vs' = Some m2.
+Proof.
+intros.
+revert vs' m m2; induction vs; intros.
+simpl.
+intuition. exists m; intuition. destruct H as [? [H ?]]; inv H; auto.
+simpl.
+case_eq (Genv.alloc_global ge m a); intros.
+specialize (IHvs vs' m0 m2).
+auto.
+intuition; try discriminate.
+destruct H0 as [? [? ?]]; discriminate.
+Qed.
+
+Fixpoint alloc_globals_rev {F V} (ge: Genv.t F V) (m: mem) (vl: list (ident * globdef F V))
+                         {struct vl} : option mem :=
+  match vl with
+  | nil => Some m
+  | v :: vl' =>
+     match alloc_globals_rev ge m vl' with
+     | Some m' => Genv.alloc_global ge m' v
+     | None => None
+     end
+  end.
+
+Lemma alloc_globals_rev_eq: 
+     forall F V (ge: Genv.t F V) m vl,
+     Genv.alloc_globals ge m (rev vl) = alloc_globals_rev ge m vl.
+Proof.
+intros.
+revert m; induction vl; intros; auto.
+simpl.
+rewrite <- IHvl.
+case_eq (Genv.alloc_globals ge m (rev vl)); intros.
+case_eq (Genv.alloc_global ge m0 a); intros.
+rewrite alloc_globals_app.
+exists m0; split; auto.
+simpl. rewrite H0; auto.
+case_eq (Genv.alloc_globals ge m (rev vl ++ a :: nil)); intros; auto.
+elimtype False.
+apply alloc_globals_app in H1.
+destruct H1 as [m' [? ?]].
+inversion2 H H1.
+simpl in H2.
+rewrite H0 in H2; inv H2.
+case_eq (Genv.alloc_globals ge m (rev vl ++ a :: nil)); intros; auto.
+elimtype False.
+apply alloc_globals_app in H0.
+destruct H0 as [m' [? ?]].
+inversion2 H H0.
+Qed.
+
+
+Lemma rev_prog_vars': forall {F V} vl, rev (@prog_vars' F V vl) = prog_vars' (rev vl).
+Proof.
+   intros.
+   induction vl. simpl; auto.
+   destruct a. destruct g.
+   simpl. rewrite IHvl.
+   clear. induction (rev vl); simpl; intros; auto. destruct a; destruct g; simpl; auto.
+    rewrite IHl. auto.
+   simpl.
+   transitivity (prog_vars' (rev vl) ++ (@prog_vars' F V ((i,Gvar v)::nil))).
+    rewrite IHvl. f_equal.
+    simpl.
+    clear.
+    induction (rev vl); simpl; intros; auto.
+    destruct a. destruct g.
+    auto.
+    rewrite <- IHl.
+    simpl. auto.
+Qed.
+
+Lemma writable_blocks_rev:
+  forall rho l, writable_blocks l rho = writable_blocks (rev l) rho.
+Proof.
+induction l; simpl; auto.
+destruct a.
+rewrite writable_blocks_app.
+rewrite <- IHl.
+simpl.
+rewrite sepcon_emp.
+apply sepcon_comm.
+Qed.
+
+Lemma add_variables_nextblock:
+  forall F V vl (ge: Genv.t F V) i g ul, list_norepet (map (@fst _ _) (vl++(i,g)::ul)) ->
+   Genv.find_symbol (Genv.add_globals ge (vl++(i,g)::ul)) i = 
+          Some (Genv.genv_next ge + Z_of_nat (length vl)).
+Proof.
+Admitted.
+
+
+Lemma global_initializers:
+  forall prog G m n,
+     list_norepet (prog_defs_names prog) ->
+    match_fdecs (prog_funct prog) G ->
+    Genv.init_mem prog = Some m ->
+     app_pred 
+      (writable_blocks (map (initblocksize type) (prog_vars prog))
+          (base.empty_environ (Genv.globalenv prog)))
+  (inflate_initial_mem m (initial_core (Genv.globalenv prog) G n)).
+Proof.
+ intros until n. intros ? SAME_IDS ?.
+ assert (IOK: initial_rmap_ok m (initial_core (Genv.globalenv prog) G n))
+      by (apply initial_core_ok; auto).
+  unfold Genv.init_mem in H0.
+  unfold Genv.globalenv in *.
+  destruct prog as [fl main vl].
+  simpl in *.
+  remember (Genv.add_globals (Genv.empty_genv fundef type) fl) as gev.
+  rewrite <- (rev_involutive fl) in *.
+  rewrite alloc_globals_rev_eq in H0.
+  forget (rev fl) as vl'. clear fl; rename vl' into vl.
+  unfold prog_vars. simpl.
+  rewrite <- rev_prog_vars'.
+  rewrite map_rev. rewrite <- writable_blocks_rev.
+  assert (exists ul, gev = Genv.add_globals (Genv.empty_genv fundef type) (rev vl ++ ul) /\ 
+                                            list_norepet (map (@fst _ _) (rev vl ++ ul))).
+  exists nil; rewrite <- app_nil_end; auto.
+  clear Heqgev H.
+  revert m H0 H1 IOK SAME_IDS; induction vl; simpl; intros.
+ apply resource_at_empty2.
+ intro l.
+ unfold inflate_initial_mem.
+ rewrite resource_at_make_rmap.
+ unfold inflate_initial_mem'.
+  inv H0.
+ unfold access_at, empty. simpl. rewrite ZMap.gi. apply NO_identity.
+(*
+ invSome.
+ destruct a; destruct g.
+ apply (H3 m0).
+ case_eq (initblocksize type a); intros.
+ specialize (IHvl _ H0).
+ unfold writable_block.
+ normalize.
+ unfold initblocksize in H.
+ destruct a. inv H.
+ unfold Genv.alloc_variable in H3.
+ simpl in H3.
+ revert H3; case_eq (alloc m0 0 (Genv.init_data_list_size (gvar_init g))); intros.
+ invSome. invSome.
+ unfold empty_environ at 1. simpl ge_of. unfold filter_genv.
+ destruct H1 as [ul [? ?]].
+ spec IHvl.
+  exists ((i,g)::ul).
+ rewrite app_ass in H1,H2; split; auto.
+ assert (Genv.find_symbol gev i = Some b).
+ clear - H0 H H1 H2 H9.
+ apply alloc_result in H. subst.
+ rewrite <- alloc_variables_rev_eq in H0. 
+ apply Genv.alloc_variables_nextblock in H0.
+ rewrite H0. clear - H2 H9.
+ rewrite app_ass in *. simpl app in *.
+ simpl nextblock. rewrite <- H9.
+ apply add_variables_nextblock; auto. 
+ rewrite H4.
+ exists (Vptr b Int.zero, match type_of_global gev b with
+      | Some t => t
+      | None => Tvoid
+      end).
+ normalize.
+ exists (b, 0).
+ normalize; exists Share.bot.
+ normalize.
+ split.
+ simpl. split.
+ destruct (type_of_global gev b); auto.
+ f_equal; rewrite Int.signed_zero; auto.
+ rewrite sepcon_comm.
+ assert (b>0). apply alloc_result in H. subst; apply nextblock_pos.
+ apply (mem_alloc_juicy _ _ _ _ _ H
+                    (initial_core gev G n)
+                   (writable_blocks (map (initblocksize type) vl) (empty_environ gev))
+                  IOK IOK) in IHvl.
+ rewrite Zminus_0_r in IHvl.
+ apply (store_zeros_lem _ _ _ _ H3 H7 _ IOK IOK) in IHvl.
+ apply (store_init_data_list_lem _ _ _ _ _ _ _ _ H5 H7 _ IOK IOK) in IHvl.
+ rewrite <- (Zminus_0_r  (Genv.init_data_list_size (gvar_init g))) in IHvl.
+ assert (Genv.perm_globvar g = Writable) by admit. (* need to generalize this! *)
+ rewrite H8 in *.
+ apply (drop_perm_writable_lem _ _ _ _ _ H6 H7 _ IOK IOK) in IHvl.
+ rewrite Zminus_0_r in IHvl.
+ apply IHvl.
+Qed. *)
+Admitted.
+
+
+Definition bump_nextvar {F V} (ge: Genv.t F V)  : Genv.t F V.
+intros.
+apply (@Genv.mkgenv F V
+    ge.(Genv.genv_symb)
+    ge.(Genv.genv_funs)
+    ge.(Genv.genv_vars)
+    (ge.(Genv.genv_next) + 1)); intros; destruct ge; simpl in *; auto.
+unfold block in *. omega.
+destruct (genv_symb_range _ _ H); split; unfold block in*; omega.
+pose proof (genv_funs_range _ _ H); omega.
+pose proof (genv_vars_range _ _ H); omega.
+eapply genv_funs_vars; eauto.
+apply genv_vars_inj with b; auto.
+Defined.
+
+Lemma disj_no_fun:
+  forall (fs: list (AST.ident * globdef fundef type)) ids, 
+       list_disjoint (map (@fst _ _) fs) ids ->
+       forall i, In i ids ->
+      (Genv.genv_symb (Genv.add_globals (Genv.empty_genv _ _) fs)) ! i = None.
+Proof.
+intros. spec H i i.
+assert (~In i (map (@fst _ _) fs)). intro. contradiction H; auto.
+clear - H1; rename H1 into H0. unfold Genv.add_globals.
+rewrite fold_right_rev_left. rewrite <- (rev_involutive fs). rewrite In_rev in H0.
+rewrite <- map_rev in H0. remember (rev fs) as fs'; rewrite rev_involutive. clear - H0.
+revert H0; induction fs'; simpl; intros.
+rewrite Maps.PTree.gempty; auto. destruct a; simpl in *.
+rewrite Maps.PTree.gso; [ | intro; subst; intuition]. 
+apply IHfs'. contradict H0; auto.
+Qed.
+
+Definition upto_block' (b: block) (w: rmap) :=
+  fun loc => if zlt (fst loc) b then w @ loc else NO Share.bot.
+
+Definition upto_block (b: block) (w: rmap) : rmap.
+ refine (proj1_sig (make_rmap (upto_block' b w) _ (level w) _)).
+Proof.
+ intros b' z'.
+ unfold compose, upto_block'.
+ simpl. destruct (zlt b' b).
+ apply rmap_valid.
+  simpl. auto.
+ extensionality loc;  unfold compose.
+  unfold upto_block'.
+ if_tac; [ | reflexivity ].
+apply resource_at_approx.
+Defined.
+
+Definition beyond_block' (b: block) (w: rmap) :=
+  fun loc => if zlt (fst loc) b then core (w @ loc) else w @ loc.
+
+Definition beyond_block (b: block) (w: rmap) : rmap.
+ refine (proj1_sig (make_rmap (beyond_block' b w) _ (level w) _)).
+Proof.
+ intros b' z'.
+ unfold compose, beyond_block'.
+ simpl. destruct (zlt b' b).
+ pose proof (rmap_valid w b' z'). unfold compose in H.
+ revert H;  case_eq (w @ (b',z')); intros;
+  repeat rewrite core_NO in *; 
+  repeat rewrite core_YES in *;
+  repeat rewrite core_PURE in *;
+   simpl; intros; auto.
+ pose proof (rmap_valid w b' z'). unfold compose in H.
+ revert H;  case_eq (w @ (b',z')); intros;
+  repeat rewrite core_NO in *; 
+  repeat rewrite core_YES in *;
+  repeat rewrite core_PURE in *;
+   simpl; intros; auto.
+ extensionality loc;  unfold compose.
+  unfold beyond_block'.
+ if_tac. repeat rewrite core_resource_at. rewrite <- level_core; apply resource_at_approx.
+apply resource_at_approx.
+Defined.
